platform/cito/Notations2.v
@@ -1,9 +1,0 @@
-Set Implicit Arguments.
-
-Require Import Notations.
-Export Notations.
-
-Infix "<-" := Syntax.Assign : stmt_scope.
-
-Notation "x <- 'Label' lbl" := (Syntax.Label x lbl)
-  (no associativity, at level 95, f at level 0) : stmt_scope.
