platform/cito/VerifCondOkNonCall2.v
@@ -38,14 +38,11 @@ Module Make (Import E : ADT) (Import M : RepInv E).
 
     Notation do_compile := (compile vars temp_size rv_postcond imports_global modName).
 
-    Require Import Notations.
     Require Import SynReqFacts.
     Require Import ListFactsNew.
     Require Import StringSet.
     Import StringSet.
     Require Import StringSetTactics.
-
-    Open Scope stmt.
 
     Opaque mult.
     Opaque star. (* necessary to use eapply_cancel *)
